src/Init/ByCases.lean
@@ -38,7 +38,7 @@ theorem apply_ite (f : α → β) (P : Prop) [Decidable P] (x y : α) :
   apply_dite f P (fun _ => x) (fun _ => y)
 
 /-- A `dite` whose results do not actually depend on the condition may be reduced to an `ite`. -/
-@[simp, auto_attach ←] theorem dite_eq_ite [Decidable P] :
+@[simp] theorem dite_eq_ite [Decidable P] :
   (dite P (fun _ => a) (fun _ => b)) = ite P a b := rfl
 
 @[deprecated "Use `ite_eq_right_iff`" (since := "2024-09-18")]
