src/Init/WF.lean
@@ -427,6 +427,6 @@ def wfParam {α : Sort u} (a : α) : α := a
 Reverse direction of `dite_eq_ite`. Used by the auto-attach feature to extend the context
 of a termination proof inside `if-then-else` with the condition.
 -/
-@[auto_attach] theorem ite_eq_dite [Decidable P] :
+@[wf_preprocess] theorem ite_eq_dite [Decidable P] :
     ite P a b = (dite P (fun h => binderNameHint h () a) (fun h => binderNameHint h () b)) := by
   rfl
